extraction/theories/WcbvEvalAux.v
@@ -1,6 +1,5 @@
 From ConCert.Extraction Require Import Aux.
 From ConCert.Extraction Require Import ClosedAux.
-From ConCert.Extraction Require Import WcbvEvalType.
 From Coq Require Import Arith.
 From Coq Require Import Bool.
 From Coq Require Import Eqdep_dec.
@@ -14,30 +13,33 @@ From MetaCoq.Erasure Require Import ECSubst.
 From MetaCoq.Erasure Require Import EInduction.
 From MetaCoq.Erasure Require Import EInversion.
 From MetaCoq.Erasure Require Import ELiftSubst.
+From MetaCoq.Erasure Require Import EWcbvEval.
 From MetaCoq.Template Require Import utils.
 
 Import ListNotations.
 Set Equations Transparent.
 
+Notation "Σ 'e⊢' s ▷ t" := (eval Σ s t) (at level 50, s, t at next level) : type_scope.
+
 Lemma eval_tApp_head Σ hd arg v :
-  Σ ⊢ tApp hd arg ▷ v ->
-  ∑ hdv, Σ ⊢ hd ▷ hdv.
+  Σ e⊢ tApp hd arg ▷ v ->
+  ∑ hdv, Σ e⊢ hd ▷ hdv.
 Proof.
   intros ev.
   now depelim ev.
 Qed.
 
 Lemma eval_tApp_arg Σ hd arg v :
-  Σ ⊢ tApp hd arg ▷ v ->
-  ∑ argv, Σ ⊢ arg ▷ argv.
+  Σ e⊢ tApp hd arg ▷ v ->
+  ∑ argv, Σ e⊢ arg ▷ argv.
 Proof.
   intros ev.
   now depelim ev.
 Qed.
 
 Lemma eval_mkApps_head Σ hd args v :
-  Σ ⊢ mkApps hd args ▷ v ->
-  ∑ hdv, Σ ⊢ hd ▷ hdv.
+  Σ e⊢ mkApps hd args ▷ v ->
+  ∑ hdv, Σ e⊢ hd ▷ hdv.
 Proof.
   revert hd v.
   induction args; intros hd v ev; [easy|].
@@ -47,7 +49,7 @@ Proof.
 Qed.
 
 Lemma eval_mkApps_args Σ hd args v :
-  Σ ⊢ mkApps hd args ▷ v ->
+  Σ e⊢ mkApps hd args ▷ v ->
   ∑ argsv, All2 (eval Σ) args argsv.
 Proof.
   revert hd v.
@@ -62,10 +64,10 @@ Proof.
 Qed.
 
 Lemma eval_tApp_heads Σ hd hd' hdv arg v :
-  Σ ⊢ hd ▷ hdv ->
-  Σ ⊢ hd' ▷ hdv ->
-  Σ ⊢ tApp hd arg ▷ v ->
-  Σ ⊢ tApp hd' arg ▷ v.
+  Σ e⊢ hd ▷ hdv ->
+  Σ e⊢ hd' ▷ hdv ->
+  Σ e⊢ tApp hd arg ▷ v ->
+  Σ e⊢ tApp hd' arg ▷ v.
 Proof.
   intros ev_hd ev_hd' ev_app.
   depind ev_app.
@@ -86,22 +88,22 @@ Derive Signature for eval.
 Derive NoConfusionHom for term.
 
 Lemma eval_tLetIn_inv Σ na val body res :
-  Σ ⊢ tLetIn na val body ▷ res ->
+  Σ e⊢ tLetIn na val body ▷ res ->
   ∑ val_res,
-    Σ ⊢ val ▷ val_res ×
-    Σ ⊢ csubst val_res 0 body ▷ res.
+    Σ e⊢ val ▷ val_res ×
+    Σ e⊢ csubst val_res 0 body ▷ res.
 Proof. intros ev; depelim ev; easy. Qed.
 
 Lemma eval_tLambda_inv Σ na body v :
-  Σ ⊢ tLambda na body ▷ v ->
+  Σ e⊢ tLambda na body ▷ v ->
   v = tLambda na body.
 Proof. now intros ev; depelim ev. Qed.
 
 Lemma eval_tApp_tLambda_inv Σ na body a v :
-  Σ ⊢ tApp (tLambda na body) a ▷ v ->
+  Σ e⊢ tApp (tLambda na body) a ▷ v ->
   ∑ av,
-    Σ ⊢ a ▷ av ×
-    Σ ⊢ csubst av 0 body ▷ v.
+    Σ e⊢ a ▷ av ×
+    Σ e⊢ csubst av 0 body ▷ v.
 Proof.
   intros ev.
   depelim ev.
@@ -118,10 +120,10 @@ Proof.
 Qed.
 
 Lemma eval_mkApps_heads Σ hd hd' hdv args v :
-  Σ ⊢ hd ▷ hdv ->
-  Σ ⊢ hd' ▷ hdv ->
-  Σ ⊢ mkApps hd args ▷ v ->
-  Σ ⊢ mkApps hd' args ▷ v.
+  Σ e⊢ hd ▷ hdv ->
+  Σ e⊢ hd' ▷ hdv ->
+  Σ e⊢ mkApps hd args ▷ v ->
+  Σ e⊢ mkApps hd' args ▷ v.
 Proof.
   revert hd hd' hdv v.
   induction args as [|a args]; intros hd hd' hdv v ev_hd ev_hd' ev.
@@ -258,7 +260,7 @@ Proof.
 Qed.
 
 Lemma eval_closed Σ t v :
-  Σ ⊢ t ▷ v ->
+  Σ e⊢ t ▷ v ->
   env_closed Σ ->
   closed t ->
   closed v.
@@ -316,7 +318,7 @@ Proof.
   - easy.
 Qed.
 
-Fixpoint deriv_length {Σ t v} (ev : Σ ⊢ t ▷ v) : nat :=
+Fixpoint deriv_length {Σ t v} (ev : Σ e⊢ t ▷ v) : nat :=
   match ev with
   | eval_atom _ _ => 1
   | red_cofix_case _ _ _ _ _ _ _ _ _ ev
@@ -335,12 +337,12 @@ Fixpoint deriv_length {Σ t v} (ev : Σ ⊢ t ▷ v) : nat :=
     S (deriv_length ev1 + deriv_length ev2 + deriv_length ev3)
   end.
 
-Lemma deriv_length_min {Σ t v} (ev : Σ ⊢ t ▷ v) :
+Lemma deriv_length_min {Σ t v} (ev : Σ e⊢ t ▷ v) :
   1 <= deriv_length ev.
 Proof. destruct ev; cbn in *; lia. Qed.
 
-Lemma eval_tApp_deriv {Σ hd arg v} (ev : Σ ⊢ tApp hd arg ▷ v) :
-  ∑ hdv (ev_hd : Σ ⊢ hd ▷ hdv) argv (ev_arg : Σ ⊢ arg ▷ argv),
+Lemma eval_tApp_deriv {Σ hd arg v} (ev : Σ e⊢ tApp hd arg ▷ v) :
+  ∑ hdv (ev_hd : Σ e⊢ hd ▷ hdv) argv (ev_arg : Σ e⊢ arg ▷ argv),
     S (deriv_length ev_hd + deriv_length ev_arg) <= deriv_length ev.
 Proof.
   depelim ev; cbn in *;
@@ -367,8 +369,8 @@ Proof.
     exact (app_All2 _ _ _ _ _ _ _ a1 a2).
 Defined.
 
-Lemma eval_mkApps_deriv {Σ hd args v} (ev : Σ ⊢ mkApps hd args ▷ v) :
-  ∑ hdv (ev_hd : Σ ⊢ hd ▷ hdv) argsv (ev_args : All2 (eval Σ) args argsv),
+Lemma eval_mkApps_deriv {Σ hd args v} (ev : Σ e⊢ mkApps hd args ▷ v) :
+  ∑ hdv (ev_hd : Σ e⊢ hd ▷ hdv) argsv (ev_args : All2 (eval Σ) args argsv),
     deriv_length ev_hd + #|args| + sum_deriv_lengths ev_args <= deriv_length ev.
 Proof.
   revert hd v ev.
@@ -381,251 +383,6 @@ Proof.
     exists (All2_cons ev_argv ev_args).
     cbn in *.
     lia.
-Qed.
-
-Lemma sum_deriv_lengths_app_All2 {Σ}
-      {ts tsv} (a : All2 (eval Σ) ts tsv)
-      {ts' tsv'} (a' : All2 (eval Σ) ts' tsv') :
-  sum_deriv_lengths (app_All2 a a') = sum_deriv_lengths a + sum_deriv_lengths a'.
-Proof.
-  induction a in ts', tsv', a' |- *; [easy|].
-  cbn in *.
-  now rewrite IHa.
-Qed.
-
-Ltac determ :=
-  repeat
-    match goal with
-    | [ev1 : ?Σ ⊢ ?t ▷ ?v, ev2 : ?Σ ⊢ ?t ▷ ?v' |- _] =>
-      match v with
-      | v' => fail 1
-      | _ => idtac
-      end;
-      match goal with
-      | [H: v = v' |- _] => fail 1
-      | [H: v' = v |- _] => fail 1
-      | _ => idtac
-      end;
-      pose proof (eval_deterministic ev1 ev2)
-    end;
-  subst.
-
-Lemma term_forall_list_rect :
-  forall P : term -> Type,
-    (P tBox) ->
-    (forall n : nat, P (tRel n)) ->
-    (forall i : ident, P (tVar i)) ->
-    (forall (n : nat) (l : list term), All P l -> P (tEvar n l)) ->
-    (forall (n : name) (t : term), P t -> P (tLambda n t)) ->
-    (forall (n : name) (t : term),
-        P t -> forall t0 : term, P t0 -> P (tLetIn n t t0)) ->
-    (forall t u : term, P t -> P u -> P (tApp t u)) ->
-    (forall s, P (tConst s)) ->
-    (forall (i : inductive) (n : nat), P (tConstruct i n)) ->
-    (forall (p : inductive * nat) (t : term),
-        P t -> forall l : list (nat * term),
-            tCaseBrsProp P l -> P (tCase p t l)) ->
-    (forall (s : projection) (t : term), P t -> P (tProj s t)) ->
-    (forall (m : mfixpoint term) (n : nat), All (fun x => P (dbody x)) m -> P (tFix m n)) ->
-    (forall (m : mfixpoint term) (n : nat), All (fun x => P (dbody x)) m -> P (tCoFix m n)) ->
-    forall t : term, P t.
-Proof.
-  intros until t. revert t.
-  fix auxt 1.
-  move auxt at top.
-  destruct t; match goal with
-                 H : _ |- _ => apply H
-              end; auto.
-  revert l.
-  fix auxl' 1.
-  destruct l; constructor; [|apply auxl'].
-  apply auxt.
-  revert l.
-  fix auxl' 1.
-  destruct l; constructor; [|apply auxl'].
-  apply auxt.
-
-  revert m.
-  fix auxm 1.
-  destruct m; constructor; [|apply auxm].
-  apply auxt.
-
-  revert m.
-  fix auxm 1.
-  destruct m; constructor; [|apply auxm].
-  apply auxt.
-Defined.
-
-(* We need UIP below *)
-Instance EqDec_term : EqDec term.
-Proof.
-  intros x.
-  induction x using term_forall_list_rect; intros []; try solve [right; discriminate].
-  - now left.
-  - destruct (eq_dec n n0); subst; [left|right]; congruence.
-  - destruct (eq_dec i i0); subst; [left|right]; congruence.
-  - destruct (eq_dec n n0); subst; [|right; congruence].
-    destruct (eq_dec #|l| #|l0|); [|right; congruence].
-    enough ({l = l0} + {l <> l0}).
-    { destruct H0; [left|right]; congruence. }
-    induction H in l0, e |- *.
-    + destruct l0; [|easy].
-      now left.
-    + destruct l0; [easy|].
-      destruct (p t); subst; [|right; congruence].
-      destruct (IHAll l0 ltac:(easy)); subst; [left|right]; congruence.
-  - destruct (eq_dec n n0); subst; [|right; congruence].
-    destruct (IHx t); subst; [left|right]; congruence.
-  - destruct (eq_dec n n0); subst; [|right; congruence].
-    destruct (IHx1 t); subst; [|right; congruence].
-    destruct (IHx2 t0); subst; [left|right]; congruence.
-  - destruct (IHx1 t); subst; [|right; congruence].
-    destruct (IHx2 t0); subst; [left|right]; congruence.
-  - destruct (eq_dec s k); subst; [left|right]; congruence.
-  - destruct (eq_dec i i0); subst; [|right; congruence].
-    destruct (eq_dec n n0); subst; [left|right]; congruence.
-  - destruct (eq_dec p p0); subst; [|right; congruence].
-    destruct (IHx t); subst; [|right; congruence].
-    destruct (eq_dec #|l| #|l0|); [|right; congruence].
-    enough ({l = l0} + {l <> l0}).
-    { destruct H; subst; [left|right]; congruence. }
-    induction X in l0, e |- *.
-    + destruct l0; [|easy].
-      now left.
-    + destruct l0; cbn in *; [easy|].
-      destruct (p p1.2); [|right; congruence].
-      destruct (eq_dec x.1 p1.1); [|right; congruence].
-      destruct (IHX l0 ltac:(easy)); subst; [|right; congruence].
-      destruct x, p1; cbn in *; subst.
-      now left.
-  - destruct (eq_dec s p); subst; [|right; congruence].
-    destruct (IHx t); [left|right]; congruence.
-  - destruct (eq_dec n n0); subst; [|right; congruence].
-    destruct (eq_dec #|m| #|m0|); [|right; congruence].
-    enough ({m = m0} + {m <> m0}).
-    { destruct H0; subst; [left|right]; congruence. }
-    induction H in m0, e |- *.
-    + destruct m0; [|easy].
-      now left.
-    + destruct m0; cbn in *; [easy|].
-      destruct (eq_dec (dname x) (dname d)); [|right; congruence].
-      destruct (p (dbody d)); [|right; congruence].
-      destruct (eq_dec (rarg x) (rarg d)); [|right; congruence].
-      destruct (IHAll m0 ltac:(easy)); subst; [|right; congruence].
-      destruct x, d; cbn in *; subst.
-      now left.
-  - destruct (eq_dec n n0); subst; [|right; congruence].
-    destruct (eq_dec #|m| #|m0|); [|right; congruence].
-    enough ({m = m0} + {m <> m0}).
-    { destruct H0; subst; [left|right]; congruence. }
-    induction H in m0, e |- *.
-    + destruct m0; [|easy].
-      now left.
-    + destruct m0; cbn in *; [easy|].
-      destruct (eq_dec (dname x) (dname d)); [|right; congruence].
-      destruct (p (dbody d)); [|right; congruence].
-      destruct (eq_dec (rarg x) (rarg d)); [|right; congruence].
-      destruct (IHAll m0 ltac:(easy)); subst; [|right; congruence].
-      destruct x, d; cbn in *; subst.
-      now left.
-Qed.
-
-Lemma deriv_lengths_eq {Σ t v} (ev1 ev2 : Σ ⊢ t ▷ v) :
-  deriv_length ev1 = deriv_length ev2.
-Proof.
-  revert ev2.
-  depind ev1; intros ev2; cbn in *.
-  - depelim ev2; cbn in *; determ; try congruence; try solve_discr.
-  - depelim ev2; cbn in *; determ; cbn in *; try congruence; try solve_discr.
-    noconf H0.
-    intuition.
-  - depelim ev2; cbn in *; determ; cbn in *; try congruence; try solve_discr.
-  - depelim ev2; cbn in *; determ; cbn in *; try congruence; try solve_discr.
-    + noconf H.
-      intuition.
-    + apply eval_mkApps_tCoFix in ev1_1 as H.
-      destruct H; solve_discr.
-  - depelim ev2; cbn in *; determ; cbn in *; try congruence; try solve_discr.
-    + noconf e0.
-      intuition.
-    + apply eval_mkApps_tCoFix in ev1_1 as H.
-      destruct H; solve_discr.
-  - depelim ev2; cbn in *; determ; cbn in *; try congruence; try solve_discr.
-    + noconf H.
-      rewrite e0 in e.
-      noconf e.
-      intuition.
-    + noconf H.
-      rewrite e0 in e.
-      noconf e.
-      lia.
-    + rewrite isFixApp_mkApps in i by easy.
-      cbn in *.
-      now rewrite Bool.orb_true_r in i.
-  - depelim ev2; cbn in *; determ; cbn in *; try congruence; try solve_discr.
-    + noconf H.
-      rewrite e0 in e.
-      noconf e.
-      lia.
-    + apply mkApps_eq_inj in e' as H'; try easy.
-      destruct H' as (H' & <-).
-      noconf H'.
-      assert (e' = eq_refl) as -> by (now apply uip).
-      cbn in *.
-      subst ev0.
-      rewrite e0 in e.
-      noconf e.
-      cbn in *.
-      intuition.
-  - depelim ev2; cbn in *; determ; cbn in *; try congruence; try solve_discr.
-    + apply eval_mkApps_tCoFix in ev2_1 as H.
-      destruct H; solve_discr.
-    + apply eval_mkApps_tCoFix in ev2_1 as H.
-      destruct H; solve_discr.
-    + apply mkApps_eq_inj in e' as H'; try easy.
-      destruct H' as (H' & <-).
-      noconf H'.
-      assert (e' = eq_refl) as -> by (now apply uip).
-      cbn in *.
-      subst ev0.
-      rewrite e0 in e.
-      noconf e.
-      cbn in *.
-      intuition.
-  - depelim ev2; cbn in *; determ; cbn in *; try congruence; try solve_discr.
-    + apply mkApps_eq_inj in e1 as H'; try easy.
-      destruct H' as (H' & <-).
-      noconf H'.
-      rewrite e0 in e.
-      noconf e.
-      assert (e1 = eq_refl) as -> by (now apply uip).
-      cbn in *.
-      subst ev0.
-      cbn in *.
-      intuition.
-    + apply eval_mkApps_tCoFix in ev2_1 as H.
-      destruct H; solve_discr.
-    + apply eval_mkApps_tCoFix in ev2 as H.
-      destruct H; solve_discr.
-  - depelim ev2; cbn in *; determ; cbn in *; try congruence; try solve_discr.
-    unfold ETyping.declared_constant in *.
-    assert (body0 = body) as -> by congruence.
-    intuition.
-  - depelim ev2; cbn in *; determ; cbn in *; try congruence; try solve_discr.
-    apply eval_mkApps_tCoFix in ev1_1 as H.
-    destruct H; solve_discr.
-  - depelim ev2; cbn in *; determ; cbn in *; try congruence; try solve_discr.
-    apply eval_mkApps_tCoFix in ev1 as H.
-    destruct H; solve_discr.
-  - depelim ev2; cbn in *; determ; cbn in *; try congruence; try solve_discr.
-    rewrite isFixApp_mkApps in i by easy.
-    cbn in *.
-    rewrite Bool.orb_true_r in i.
-    now cbn in *.
-  - depelim ev2; cbn in *; determ; cbn in *; try congruence; try solve_discr.
-    assert (e = eq_refl) as -> by (now apply uip).
-    cbn in *.
-    now subst ev0.
 Qed.
 
 Lemma All2_split_eq
@@ -674,7 +431,7 @@ Inductive All2_eval_app_spec Σ : list term -> term ->
                                  list term -> term ->
                                  forall ts tsv, All2 (eval Σ) ts tsv -> Type :=
 | All2_eval_app_intro {ts tsv} (a : All2 (eval Σ) ts tsv)
-                      {x xv} (evx : Σ ⊢ x ▷ xv) :
+                      {x xv} (evx : Σ e⊢ x ▷ xv) :
     All2_eval_app_spec
       Σ ts x tsv xv
       (ts ++ [x])
@@ -698,48 +455,42 @@ Proof.
 Qed.
 
 Lemma eval_tApp_heads_deriv {Σ hd hd' hdv arg v}
-      (ev_hd : Σ ⊢ hd ▷ hdv)
-      (ev_hd' : Σ ⊢ hd' ▷ hdv)
-      (ev_app : Σ ⊢ tApp hd arg ▷ v) :
-  ∑ (ev_app' : Σ ⊢ tApp hd' arg ▷ v),
+      (ev_hd : Σ e⊢ hd ▷ hdv)
+      (ev_hd' : Σ e⊢ hd' ▷ hdv)
+      (ev_app : Σ e⊢ tApp hd arg ▷ v) :
+  ∑ (ev_app' : Σ e⊢ tApp hd' arg ▷ v),
     (deriv_length ev_app + deriv_length ev_hd' = deriv_length ev_app' + deriv_length ev_hd)%nat.
 Proof.
   depind ev_app.
-  - pose proof (eval_deterministic ev_hd ev_app1) as ->.
-    pose proof (deriv_lengths_eq ev_hd ev_app1).
+  - pose proof (eval_unique_sig ev_hd ev_app1) as H; noconf H.
     unshelve eexists _; [now eapply eval_box|].
     cbn; lia.
-  - pose proof (eval_deterministic ev_hd ev_app1) as ->.
-    pose proof (deriv_lengths_eq ev_hd ev_app1).
+  - pose proof (eval_unique_sig ev_hd ev_app1) as H; noconf H.
     unshelve eexists _; [now eapply eval_beta|].
     cbn; lia.
-  - pose proof (eval_deterministic ev_hd ev_app1) as ->.
-    pose proof (deriv_lengths_eq ev_hd ev_app1).
+  - pose proof (eval_unique_sig ev_hd ev_app1) as H; noconf H.
     unshelve eexists _; [now eapply eval_fix|].
     cbn; lia.
-  - pose proof (eval_deterministic ev_hd ev_app1) as ->.
-    pose proof (deriv_lengths_eq ev_hd ev_app1).
+  - pose proof (eval_unique_sig ev_hd ev_app1) as H; noconf H.
     unshelve eexists _; [now eapply eval_fix_value|].
     cbn; lia.
-  - pose proof (eval_deterministic ev_hd ev_app1) as ->.
-    pose proof (deriv_lengths_eq ev_hd ev_app1).
+  - pose proof (eval_unique_sig ev_hd ev_app1) as H; noconf H.
     unshelve eexists _; [now eapply eval_app_cong|].
     cbn; lia.
   - easy.
 Qed.
 
 Lemma eval_mkApps_heads_deriv {Σ hd hd' hdv args v}
-      (ev_hd : Σ ⊢ hd ▷ hdv)
-      (ev_hd' : Σ ⊢ hd' ▷ hdv)
-      (ev_apps : Σ ⊢ mkApps hd args ▷ v) :
-  ∑ (ev_apps' : Σ ⊢ mkApps hd' args ▷ v),
+      (ev_hd : Σ e⊢ hd ▷ hdv)
+      (ev_hd' : Σ e⊢ hd' ▷ hdv)
+      (ev_apps : Σ e⊢ mkApps hd args ▷ v) :
+  ∑ (ev_apps' : Σ e⊢ mkApps hd' args ▷ v),
   (deriv_length ev_apps + deriv_length ev_hd' = deriv_length ev_apps' + deriv_length ev_hd)%nat.
 Proof.
   revert hd hd' hdv v ev_hd ev_hd' ev_apps.
   induction args using MCList.rev_ind; intros; cbn in *.
-  - pose proof (eval_deterministic ev_hd ev_apps) as ->.
-    exists ev_hd'.
-    now pose proof (deriv_lengths_eq ev_hd ev_apps).
+  - pose proof (eval_unique_sig ev_hd ev_apps) as H; noconf H.
+    exists ev_hd'; lia.
   - revert ev_apps; rewrite !mkApps_app; intros.
     cbn in *.
     eapply eval_tApp_head in ev_apps as ev_apps'.
