extraction/theories/ErasureCorrectness.v
@@ -1,15 +1,14 @@
 From ConCert.Extraction Require Import ClosedAux.
 From ConCert.Extraction Require Import Erasure.
 From ConCert.Extraction Require Import Extraction.
-From ConCert.Extraction Require Import MetaCoqErasureCorrectnessStrong.
 From ConCert.Extraction Require Import Optimize.
 From ConCert.Extraction Require Import OptimizeCorrectness.
 From ConCert.Extraction Require Import ResultMonad.
-From ConCert.Extraction Require Import WcbvEvalType.
 From Coq Require Import List.
 From Coq Require Import Permutation.
 From Coq Require Import String.
 From Equations Require Import Equations.
+From MetaCoq.Erasure Require Import EDeps.
 From MetaCoq.Erasure Require Import ErasureCorrectness.
 From MetaCoq.Erasure Require Import ErasureFunction.
 From MetaCoq.Erasure Require Import ESubstitution.
@@ -34,7 +33,6 @@ Module P := PCUICAst.
 Module E := EAst.
 
 Notation "Σ 'p⊢' s ▷ t" := (PCUICWcbvEval.eval Σ s t) (at level 50, s, t at next level) : type_scope.
-Notation "Σ 'e⊢' s ▷ t" := (EWcbvEval.eval Σ s t) (at level 50, s, t at next level) : type_scope.
 
 Lemma contains_In k ks :
   Erasure.contains k ks <-> In k ks.
@@ -62,83 +60,6 @@ Proof.
     now apply contains_In in cont.
 Qed.
 
-Lemma erases_deps_forall_ind Σ Σ'
-  (P : Extract.E.term -> Prop)
-  (Hbox : P Extract.E.tBox)
-  (Hrel : forall i : nat, P (Extract.E.tRel i))
-  (Hvar : forall n : ident, P (Extract.E.tVar n))
-  (Hevar :
-     forall (m : nat) (l : list Extract.E.term),
-       Forall P l ->
-       Forall (erases_deps Σ Σ') l -> P (Extract.E.tEvar m l))
-  (Hlam : forall (na : name) (body : Extract.E.term),
-        erases_deps Σ Σ' body -> P body -> P (Extract.E.tLambda na body))
-  (Hletin : forall (na : name) (val body : Extract.E.term),
-        erases_deps Σ Σ' val ->
-        P val -> erases_deps Σ Σ' body -> P body -> P (Extract.E.tLetIn na val body))
-  (Happ : forall hd arg : Extract.E.term,
-        erases_deps Σ Σ' hd -> P hd -> erases_deps Σ Σ' arg -> P arg -> P (Extract.E.tApp hd arg))
-  (Hconst : forall (kn : kername) (cb : PCUICAst.PCUICEnvironment.constant_body) (cb' : EAst.constant_body),
-      declared_constant Σ kn cb ->
-      ETyping.declared_constant Σ' kn cb' ->
-      erases_constant_body (Σ, PCUICAst.cst_universes cb) cb cb' ->
-      (forall body : Extract.E.term, Extract.E.cst_body cb' = Some body -> erases_deps Σ Σ' body) ->
-      (forall body : Extract.E.term, Extract.E.cst_body cb' = Some body -> P body) ->
-        P (Extract.E.tConst kn))
-  (Hconstruct : forall (ind : inductive) (c : nat), P (Extract.E.tConstruct ind c))
-  (Hcase : forall (p : inductive × nat) (discr : Extract.E.term) (brs : list (nat × Extract.E.term)),
-        erases_deps Σ Σ' discr ->
-        P discr ->
-        Forall (fun br : nat × Extract.E.term => erases_deps Σ Σ' br.2) brs ->
-        Forall (fun br => P br.2) brs ->
-        P (Extract.E.tCase p discr brs))
-  (Hproj : forall (p : projection) (t : Extract.E.term),
-        erases_deps Σ Σ' t -> P t -> P (Extract.E.tProj p t))
-  (Hfix : forall (defs : list (Extract.E.def Extract.E.term)) (i : nat),
-         Forall (fun d : Extract.E.def Extract.E.term => erases_deps Σ Σ' (Extract.E.dbody d)) defs ->
-         Forall (fun d => P (E.dbody d)) defs ->
-         P (Extract.E.tFix defs i))
-  (Hcofix : forall (defs : list (Extract.E.def Extract.E.term)) (i : nat),
-         Forall (fun d : Extract.E.def Extract.E.term => erases_deps Σ Σ' (Extract.E.dbody d)) defs ->
-         Forall (fun d => P (E.dbody d)) defs ->
-         P (Extract.E.tCoFix defs i)) :
-  forall t, erases_deps Σ Σ' t -> P t.
-Proof.
-  fix f 2.
-  intros t ed.
-  move f at top.
-  destruct ed;
-    try solve [match goal with
-    | [H: _ |- _] => apply H
-    end; auto].
-  - apply Hevar; [|assumption].
-    revert l H.
-    fix f' 2.
-    intros l [].
-    + now constructor.
-    + constructor; [now apply f|now apply f'].
-  - eapply Hconst; try eassumption.
-    intros.
-    apply f.
-    now apply H2.
-  - apply Hcase; try assumption.
-    + now apply f.
-    + revert brs H.
-      fix f' 2.
-      intros brs []; [now constructor|].
-      constructor; [now apply f|now apply f'].
-  - apply Hfix; try assumption.
-    revert defs H.
-    fix f' 2.
-    intros defs []; [now constructor|].
-    constructor; [now apply f|now apply f'].
-  - apply Hcofix; try assumption.
-    revert defs H.
-    fix f' 2.
-    intros defs []; [now constructor|].
-    constructor; [now apply f|now apply f'].
-Defined.
-
 Lemma erases_deps_cons_left Σ Σ' kn decl t :
   wf ((kn, decl) :: Σ) ->
   erases_deps Σ Σ' t ->
@@ -155,55 +76,6 @@ Proof.
     destruct kername_eq_dec as [<-|]; [congruence|].
     eassumption.
   - eassumption.
-  - unfold erases_constant_body in *.
-    destruct PCUICAst.cst_body eqn:body.
-    + destruct E.cst_body eqn:ebody; [|easy].
-      assert (declared_constant ((kn, decl) :: Σ) kn0 cb).
-      { unfold declared_constant.
-        cbn.
-        unfold eq_kername.
-        inversion wfΣ; subst.
-        destruct kername_eq_dec as [<-|]; [congruence|].
-        easy. }
-      inversion wfΣ; subst.
-      eapply PCUICWeakeningEnv.declared_constant_inv in H4; eauto.
-      2:eapply PCUICWeakeningEnv.weaken_env_prop_typing.
-      red in H4.
-      rewrite body in *.
-      cbn in *.
-      eapply (erases_extends (_, P.cst_universes cb)); eauto.
-      2: eexists [_]; reflexivity.
-      eapply declared_constant_inv in H.
-      2:eapply PCUICWeakeningEnv.weaken_env_prop_typing.
-      2: easy.
-      2: easy.
-      unfold on_constant_decl in H.
-      rewrite body in *.
-      apply H.
-    + now destruct E.cst_body.
-  - easy.
-Qed.
-
-Lemma erases_deps_cons Σ Σ' kn decl decl' t :
-  wf ((kn, decl) :: Σ) ->
-  erases_deps Σ Σ' t ->
-  erases_deps ((kn, decl) :: Σ) ((kn, decl') :: Σ') t.
-Proof.
-  intros wfΣ er.
-  induction er using erases_deps_forall_ind; try solve [now constructor].
-  apply lookup_env_Some_fresh in H as not_fresh.
-  econstructor.
-  - unfold declared_constant in *.
-    cbn.
-    unfold eq_kername.
-    inversion wfΣ; subst.
-    destruct kername_eq_dec as [<-|]; [congruence|].
-    eassumption.
-  - unfold ETyping.declared_constant in *.
-    cbn.
-    inversion wfΣ; subst.
-    destruct kername_eq_dec; [congruence|].
-    eassumption.
   - unfold erases_constant_body in *.
     destruct PCUICAst.cst_body eqn:body.
     + destruct E.cst_body eqn:ebody; [|easy].
@@ -281,7 +153,7 @@ Proof.
   induction t in ks, t, isin |- * using EInduction.term_forall_list_ind; cbn in *; auto.
   - induction H in ks, isin |- *; [easy|].
     cbn in *.
-    now apply IHForall.
+    now apply IHAll.
   - now apply In_add_seen.
   - now apply In_add_seen.
   - destruct p.
@@ -294,10 +166,10 @@ Proof.
     now apply IHt, In_add_seen.
   - apply In_fold_left; [easy|].
     intros.
-    now eapply Forall_All, All_In in H as [H]; [|eassumption].
+    now eapply All_In in H as [H]; [|eassumption].
   - apply In_fold_left; [easy|].
     intros.
-    now eapply Forall_All, All_In in H as [H]; [|eassumption].
+    now eapply All_In in H as [H]; [|eassumption].
 Qed.
 
 Lemma In_fold_left_new_exists {A} k (ks : list kername) f (ts : list A) :
@@ -364,7 +236,7 @@ Proof.
     + intros.
       now apply In_Eterm_deps_already.
     + intros.
-      now eapply Forall_All, All_In in H as [H]; [|eassumption].
+      now eapply All_In in H as [H]; [|eassumption].
   - destruct (contains k (Eterm_deps ks t1)) eqn:cont.
     + apply contains_In in cont.
       now apply In_Eterm_deps_already.
@@ -408,12 +280,12 @@ Proof.
     + intros.
       now apply In_Eterm_deps_already.
     + intros.
-      now eapply Forall_All, All_In in H as [H]; [|eassumption].
+      now eapply All_In in H as [H]; [|eassumption].
   - eapply In_fold_left_new; eauto.
     + intros.
       now apply In_Eterm_deps_already.
     + intros.
-      now eapply Forall_All, All_In in H as [H]; [|eassumption].
+      now eapply All_In in H as [H]; [|eassumption].
 Qed.
 
 Lemma In_fold_box_type_deps k ks ts :
@@ -445,107 +317,6 @@ Proof.
   - destruct p.
     now apply In_box_type_deps.
 Qed.
-
-Lemma erases_forall_list_ind
-      Σ (P : P.context -> P.term -> E.term -> Prop)
-(Hrel : forall (Γ : P.context) (i : nat), P Γ (P.tRel i) (E.tRel i))
-(Hvar : forall (Γ : P.context) (n : ident), P Γ (P.tVar n) (E.tVar n))
-(Hevar : forall (Γ : P.context) (m m' : nat) (l : list P.term) (l' : list E.term),
- All2 (erases Σ Γ) l l' ->
- Forall2 (P Γ) l l' ->
- P Γ (P.tEvar m l) (E.tEvar m' l'))
-(Hlam : forall (Γ : P.context) (na : name) (b t : P.term) (t' : E.term),
- Σ;;; (P.vass na b :: Γ) |- t ⇝ℇ t' ->
- P (P.vass na b :: Γ) t t' -> P Γ (P.tLambda na b t) (E.tLambda na t'))
-(Hletin : forall (Γ : P.context) (na : name) (t1 : P.term) (t1' : E.term)
-   (T t2 : P.term) (t2' : E.term),
- Σ;;; Γ |- t1 ⇝ℇ t1' ->
- P Γ t1 t1' ->
- Σ;;; (P.vdef na t1 T :: Γ) |- t2 ⇝ℇ t2' ->
- P (P.vdef na t1 T :: Γ) t2 t2' ->
- P Γ (P.tLetIn na t1 T t2) (E.tLetIn na t1' t2'))
-(Happ : forall (Γ : P.context) (f4 u : P.term) (f' u' : E.term),
- Σ;;; Γ |- f4 ⇝ℇ f' ->
- P Γ f4 f' -> Σ;;; Γ |- u ⇝ℇ u' -> P Γ u u' -> P Γ (P.tApp f4 u) (E.tApp f' u'))
-(Hconst : forall (Γ : P.context) (kn : kername) (u : Universes.Instance.t),
- P Γ (P.tConst kn u) (E.tConst kn))
-(Hconstruct : forall (Γ : P.context) (kn : inductive) (k : nat) (n : Universes.Instance.t),
- P Γ (P.tConstruct kn k n) (E.tConstruct kn k))
-(Hcase : forall (Γ : P.context) (ind : inductive) (npar : nat) (T c : P.term)
-   (brs : list (nat × P.term)) (c' : E.term) (brs' : list (nat × E.term)),
- PCUICElimination.Informative Σ ind ->
- Σ;;; Γ |- c ⇝ℇ c' ->
- P Γ c c' ->
- All2
-   (fun (x : nat × P.term) (x' : nat × E.term) => Σ;;; Γ |- x.2 ⇝ℇ x'.2 × x.1 = x'.1)
-   brs brs' ->
-Forall2 (fun br br' => P Γ br.2 br'.2) brs brs' ->
- P Γ (P.tCase (ind, npar) T c brs) (E.tCase (ind, npar) c' brs'))
-(Hproj : forall (Γ : P.context) (p : (inductive × nat) × nat) (c : P.term)
-   (c' : E.term),
- let ind := p.1.1 in
- PCUICElimination.Informative Σ ind ->
- Σ;;; Γ |- c ⇝ℇ c' -> P Γ c c' -> P Γ (P.tProj p c) (E.tProj p c'))
-(Hfix : forall (Γ : P.context) (mfix : mfixpoint P.term) (n : nat)
-   (mfix' : list (E.def E.term)),
- All2
-   (fun (d : def P.term) (d' : E.def E.term) =>
-    dname d = E.dname d'
-    × rarg d = E.rarg d'
-      × Σ;;; P.app_context Γ (PCUICLiftSubst.fix_context mfix) |-
-        dbody d ⇝ℇ E.dbody d') mfix mfix' ->
- Forall2 (fun d d' => P (P.app_context Γ (PCUICLiftSubst.fix_context mfix)) (dbody d) (EAst.dbody d') ) mfix mfix' ->
- P Γ (P.tFix mfix n) (E.tFix mfix' n))
-(Hcofix : forall (Γ : P.context) (mfix : mfixpoint P.term) (n : nat)
-   (mfix' : list (E.def E.term)),
- All2
-   (fun (d : def P.term) (d' : E.def E.term) =>
-    dname d = E.dname d'
-    × rarg d = E.rarg d'
-      × Σ;;; P.app_context Γ (PCUICLiftSubst.fix_context mfix) |-
-        dbody d ⇝ℇ E.dbody d') mfix mfix' ->
- Forall2 (fun d d' => P (P.app_context Γ (PCUICLiftSubst.fix_context mfix)) (dbody d) (EAst.dbody d') ) mfix mfix' ->
- P Γ (P.tCoFix mfix n) (E.tCoFix mfix' n))
-(Hbox : forall (Γ : P.context) (t : P.term), isErasable Σ Γ t -> P Γ t E.tBox) :
-  forall (Γ : P.context) (t : P.term) (t0 : E.term),
-    Σ;;; Γ |- t ⇝ℇ t0 -> P Γ t t0.
-Proof.
-  fix f 4.
-  intros Γ t et er.
-  move f at top.
-  destruct er;
-    try solve [match goal with
-    | [H: _ |- _] => apply H
-    end; auto].
-  - apply Hevar; [assumption|].
-    revert l l' X.
-    fix f' 3.
-    intros l l' [].
-    + now constructor.
-    + constructor; [now apply f|now apply f'].
-  - apply Hcase; try assumption.
-    + now apply f.
-    + revert brs brs' X.
-      fix f' 3.
-      intros brs brs' []; [now constructor|].
-      constructor; [now apply f|now apply f'].
-  - apply Hfix; try assumption.
-    revert X.
-    generalize mfix at 1 3.
-    intros mfix_gen.
-    revert mfix mfix'.
-    fix f' 3.
-    intros mfix mfix' []; [now constructor|].
-    constructor; [now apply f|now apply f'].
-  - apply Hcofix; try assumption.
-    revert X.
-    generalize mfix at 1 3.
-    intros mfix_gen.
-    revert mfix mfix'.
-    fix f' 3.
-    intros mfix mfix' []; [now constructor|].
-    constructor; [now apply f|now apply f'].
-Defined.
 
 Lemma erases_deps_recursive Σ Σer t T et :
   wf_ext Σ ->
@@ -713,14 +484,9 @@ Proof.
 Qed.
 
 Opaque erase_type SafeErasureFunction.wf_reduction.
-Lemma erase_global_decls_deps_recursive_correct Σ wfΣ include ignore erase_func Σex :
+Lemma erase_global_decls_deps_recursive_correct Σ wfΣ include ignore Σex :
   (forall k, ignore k = false) ->
-  (forall Σ Γ t T wfΣ t',
-      Σ;;; Γ |- t : T ->
-      forall wt,
-        erase_func Σ wfΣ Γ t wt = PCUICSafeChecker.Checked t' ->
-        Σ;;; Γ |- t ⇝ℇ t') ->
-  erase_global_decls_deps_recursive erase_func Σ wfΣ include ignore = Ok Σex ->
+  erase_global_decls_deps_recursive Σ wfΣ include ignore = Ok Σex ->
   (forall k,
       In k include ->
       match P.lookup_env Σ k with
@@ -729,16 +495,16 @@ Lemma erase_global_decls_deps_recursive_correct Σ wfΣ include ignore erase_fun
       | _ => True
       end).
 Proof.
-  intros no_ignores erase_erases er.
+  intros no_ignores er.
   induction Σ as [|(kn, decl) Σ IH] in wfΣ, include, Σex, er |- *; [easy|].
   simpl in *.
   match goal with
-  | [H: context[erase_global_decl _ _ ?wfΣarg _ _ ?wfdeclarg] |- _] =>
+  | [H: context[erase_global_decl _ ?wfΣarg _ _ ?wfdeclarg] |- _] =>
       set (wfΣext := wfΣarg) in *; clearbody wfΣext;
         set (wfdecl := wfdeclarg) in *; clearbody wfdecl
   end.
   match goal with
-  | [H: context[erase_global_decls_deps_recursive _ _ ?wfΣarg] |- _] =>
+  | [H: context[erase_global_decls_deps_recursive _ ?wfΣarg] |- _] =>
     set (wfΣprev := wfΣarg) in *; clearbody wfΣprev
   end.
 
@@ -823,14 +589,16 @@ Proof.
           cbn in *.
           congruence. }
 
-      destruct erase_func eqn:er; cbn in *; [|congruence].
+      match goal with
+      | [H: context[SafeErasureFunction.erase _ _ _ _ ?p] |- _] =>
+        set (twt := p) in *; clearbody twt
+      end.
       inversion erconst; subst; clear erconst.
       inversion erdecl; subst; clear erdecl.
       cbn in *.
       specialize (IH _ _ _ errec).
       destruct wfΣ as [wfΣ].
       destruct wfdecl as [wfdecl].
-      eapply erase_erases in er; eauto.
       econstructor.
       * unfold declared_constant; cbn; rewrite eq_kername_refl; reflexivity.
       * unfold ETyping.declared_constant; cbn.
@@ -840,17 +608,18 @@ Proof.
         eapply type_reduction in wfdecl; eauto.
         2: now inversion wfΣ.
         eapply (erases_extends (_, _)).
-        2: eauto.
+        2: now eauto.
         1: now inversion wfΣ.
         2: eexists [_]; reflexivity.
-        2: eauto.
-        eauto.
+        1: now eauto.
+        apply SafeErasureFunction.erases_erase.
       * intros.
         cbn in *.
         noconf H.
         destruct wfΣext.
         apply erases_deps_cons; eauto.
         eapply (erases_deps_recursive (Σ, cst_universes)); eauto.
+        { apply SafeErasureFunction.erases_erase. }
         intros.
         apply IH.
         apply In_box_type_deps.
