extraction/theories/ExtractionCorrectness.v
@@ -3,15 +3,15 @@ From ConCert.Extraction Require Import ClosedAux.
 From ConCert.Extraction Require Import Erasure.
 From ConCert.Extraction Require Import ErasureCorrectness.
 From ConCert.Extraction Require Import Extraction.
-From ConCert.Extraction Require Import MetaCoqErasureCorrectnessStrong.
 From ConCert.Extraction Require Import Optimize.
 From ConCert.Extraction Require Import OptimizeCorrectness.
 From ConCert.Extraction Require Import ResultMonad.
-From ConCert.Extraction Require Import WcbvEvalType.
+From ConCert.Extraction Require Import WcbvEvalAux.
 From Coq Require Import Arith.
 From Coq Require Import List.
 From Coq Require Import String.
 From Equations Require Import Equations.
+From MetaCoq.Erasure Require Import ErasureCorrectness.
 From MetaCoq.Erasure Require Import ErasureFunction.
 From MetaCoq.Erasure Require Import EWcbvEval.
 From MetaCoq.Erasure Require Import Extract.
@@ -31,7 +31,6 @@ Module P := PCUICAst.
 Module E := EAst.
 
 Notation "Σ 'p⊢' s ▷ t" := (PCUICWcbvEval.eval Σ s t) (at level 50, s, t at next level) : type_scope.
-Notation "Σ 'e⊢' s ▷ t" := (EWcbvEval.eval Σ s t) (at level 50, s, t at next level) : type_scope.
 
 Lemma eval_const_construct_mask Σ kn ind c im cm :
   trans_env Σ e⊢ E.tConst kn ▷ E.tConstruct ind c ->
@@ -48,7 +47,7 @@ Proof.
     now destruct get_const_mask. }
   eapply nth_error_forall in nth; [|eassumption].
   cbn in *.
-  rewrite H in nth.
+  rewrite e in nth.
   propify.
   destruct nth as (valid_mask_body & _).
   clear -ev valid_mask_body.
@@ -78,7 +77,7 @@ Theorem extract_correct
   extract_pcuic_env
     (pcuic_args extract_within_coq)
     Σ (wf_ext_wf_squash wfΣ) [kn] ignored = Ok exΣ ->
-  trans_env exΣ e⊢ E.tConst kn ▷ E.tConstruct ind c.
+  ∥trans_env exΣ e⊢ E.tConst kn ▷ E.tConstruct ind c∥.
 Proof.
   intros ax [T wt] ev not_erasable no_ignores ex.
   cbn in *.
@@ -90,21 +89,18 @@ Proof.
   inversion_clear ex.
   rewrite trans_env_debox_env_types.
   eapply erase_global_decls_deps_recursive_correct in er; eauto.
-  3: left; reflexivity.
-  2: intros.
-  2: now eapply SafeErasureFunction.erases_erase.
+  2: left; reflexivity.
   assert (ev' := ev).
   depelim ev'.
   unfold declared_constant in isdecl.
   rewrite isdecl in er.
 
-  eapply erases_correct in er as (erv & erase_to & erev); eauto.
+  eapply erases_correct in er as (erv & erase_to & [erev]); eauto.
   2: now constructor.
 
   depelim erase_to; [|easy].
 
   eapply eval_const_construct_mask in erev as no_mask; eauto.
-  apply eval_evalT in erev as [erev].
   assert (ctor_exp := erev).
   eapply eval_is_expanded_aux with (k := 0) in ctor_exp; eauto.
   2: now cbn; rewrite no_mask.
@@ -114,7 +110,7 @@ Proof.
     rewrite no_mask in erev.
     destruct get_ctor_mask; [|easy].
     cbn in *.
-    now apply evalT_eval.
+    now constructor.
   - cbn.
     now rewrite no_mask.
 Qed.
@@ -122,18 +118,14 @@ Qed.
 Print Assumptions extract_correct.
 
 (* There are some assumptions of which almost all are in MetaCoq.
-   There are three assumptions in the list from this project.
+   From this project are the following:
 
-   1. metacoq_cofix_erasure_is_admitted, used in from MetaCoqErasureCorrectnessStrong.v.
-      This admission comes from the original MetaCoq development from which the proof was
-      adapted to be stronger. Since we do not extract cofixes this does not matter much.
-
-   2. hnf_completion, which is used in flag_of_type. These cases require a completion
+   1. hnf_completion, which is used in flag_of_type. These cases require a completion
       statement about the hnf function from MetaCoq, saying that this function actually
       reduces to head normal from. MetaCoq does not yet include a completeness statement
       about hnf (but it is planned), so for now we defer those proofs.
 
-   3. assume_env_wellformed, which is used to assume that the environments we extract are
+   2. assume_env_wellformed, which is used to assume that the environments we extract are
       wellformed. MetaCoq's safe checker does not run from within Coq, so we cannot type
       check the environments. However, our environments are unquoted directly from Coq's
       kernel where they are already welltyped, so this is justified (and the same assumption
